SafetyOracles.thy
@@ -13,47 +13,47 @@ fun later :: "(message * message) \<Rightarrow> bool"
     "later (m1, m2) = (m2 \<in> justification m1)"
 
 (* Definition 7.2 *)
-fun from_sender :: "(validator * state) \<Rightarrow> message set"
+fun from_sender :: "params \<Rightarrow> (validator * state) \<Rightarrow> message set"
   where
-    "from_sender (v, \<sigma>) = {m. m \<in> \<sigma> \<and> sender m = v}"
+    "from_sender params (v, \<sigma>) = {m \<in> M params. m \<in> \<sigma> \<and> sender m = v}"
      
 (* Definition 7.3 *)
-fun later_from :: "(message * validator * state) \<Rightarrow> message set"
+fun later_from :: "params \<Rightarrow> (message * validator * state) \<Rightarrow> message set"
   where
-    "later_from (m, v, \<sigma>) = {m'. m \<in> \<sigma> \<and> sender m' = v \<and> later (m', m)}"
+    "later_from params (m, v, \<sigma>) = {m' \<in> M params. m \<in> \<sigma> \<and> sender m' = v \<and> later (m', m)}"
  
 (* Definition 7.4 *)
-fun latest_messages :: "(state * validator) \<Rightarrow> message set"
+fun latest_messages :: "params \<Rightarrow> (state * validator) \<Rightarrow> message set"
   where
-    "latest_messages (\<sigma>, v) = {m. m \<in> \<sigma> \<and> sender m = v \<and> later_from (m, v, \<sigma>) = \<emptyset>}"
+    "latest_messages params (\<sigma>, v) = {m \<in> M params. m \<in> \<sigma> \<and> sender m = v \<and> later_from params (m, v, \<sigma>) = \<emptyset>}"
 
 (* Definition 7.5 *)
-fun latest_messages_from_honest_validators :: "(state *validator) \<Rightarrow> message set"
+fun latest_messages_from_honest_validators :: "params \<Rightarrow> (state *validator) \<Rightarrow> message set"
   where
-    "latest_messages_from_honest_validators (\<sigma>, v) = 
-      (if v \<in> equivocating_validators \<sigma> then \<emptyset> else latest_messages (\<sigma>, v))"
+    "latest_messages_from_honest_validators params (\<sigma>, v) = 
+      (if v \<in> equivocating_validators params \<sigma> then \<emptyset> else latest_messages params (\<sigma>, v))"
 
 (* Definition 7.6 *)
-fun latest_estimates_from_honest_validators :: "(state * validator) \<Rightarrow> consensus_value set"
+fun latest_estimates_from_honest_validators :: "params \<Rightarrow> (state * validator) \<Rightarrow> consensus_value set"
   where
-    "latest_estimates_from_honest_validators (\<sigma>, v) = 
-      {est m | m. m \<in> latest_messages_from_honest_validators (\<sigma>, v)}"
+    "latest_estimates_from_honest_validators params (\<sigma>, v) = 
+      {est m | m. m \<in> latest_messages_from_honest_validators params (\<sigma>, v)}"
 
 (* Definition 7.7 *)
-fun latest_justifications_from_honest_validators :: "(state * validator) \<Rightarrow> state set"
+fun latest_justifications_from_honest_validators :: "params \<Rightarrow> (state * validator) \<Rightarrow> state set"
   where
-    "latest_justifications_from_honest_validators (\<sigma>, v) = 
-      {justification m | m. m \<in> latest_messages_from_honest_validators (\<sigma>, v)}"
+    "latest_justifications_from_honest_validators params (\<sigma>, v) = 
+      {justification m | m. m \<in> latest_messages_from_honest_validators params (\<sigma>, v)}"
 
 (* Definition 7.8 *)
-fun agreeing_validators :: "(consensus_value_property * state) \<Rightarrow> validator set"
+fun agreeing_validators :: "params \<Rightarrow> (consensus_value_property * state) \<Rightarrow> validator set"
   where
-    "agreeing_validators (p, \<sigma>) = {v. \<forall> c. c \<in> latest_estimates_from_honest_validators (\<sigma>, v) \<and> p c}"
+    "agreeing_validators params (p, \<sigma>) = {v \<in> V params. \<forall> c \<in> C params. c \<in> latest_estimates_from_honest_validators params (\<sigma>, v) \<and> p c}"
 
 (* Definition 7.9 *)
-fun disagreeing_validators :: "(consensus_value_property * state) \<Rightarrow> validator set"
+fun disagreeing_validators :: "params \<Rightarrow> (consensus_value_property * state) \<Rightarrow> validator set"
   where
-    "disagreeing_validators (p, \<sigma>) = {v. \<exists> c. c \<in> latest_estimates_from_honest_validators (\<sigma>, v) \<and> \<not> p c}"
+    "disagreeing_validators params (p, \<sigma>) = {v \<in> V params. \<exists> c \<in> C params. c \<in> latest_estimates_from_honest_validators params (\<sigma>, v) \<and> \<not> p c}"
 
 (* Definition 7.10 *)
 definition weight_measure :: "params \<Rightarrow> validator set \<Rightarrow> real"
@@ -63,23 +63,25 @@ definition weight_measure :: "params \<Rightarrow> validator set \<Rightarrow> r
 (* Definition 7.11 *)
 fun is_majority :: "params \<Rightarrow> (validator set * state) \<Rightarrow> bool"
   where
-    "is_majority params (v_set, \<sigma>) = (weight_measure params v_set > (weight_measure params (V params) - weight_measure params (equivocating_validators \<sigma>)) div 2)"
+    "is_majority params (v_set, \<sigma>) = 
+      (weight_measure params v_set > (weight_measure params (V params) - weight_measure params (equivocating_validators params \<sigma>)) div 2)"
    
 (* Definition 7.12 *)
 definition is_majority_driven :: "params \<Rightarrow> consensus_value_property \<Rightarrow> bool"
   where
-    "is_majority_driven params p = (\<forall> \<sigma> c. \<sigma> \<in> \<Sigma> params \<and> is_majority params (agreeing_validators (p, \<sigma>), \<sigma>) \<longrightarrow> c \<in> \<epsilon> params \<sigma> \<and> p c)"
+    "is_majority_driven params p = (\<forall> \<sigma> \<in> \<Sigma> params. is_majority params (agreeing_validators params (p, \<sigma>), \<sigma>) \<longrightarrow> (\<forall> c \<in> \<epsilon> params \<sigma>. p c))"
 
 (* Definition 7.13 *)
 definition is_max_driven :: "params \<Rightarrow> consensus_value_property \<Rightarrow> bool"
   where
     "is_max_driven params p =
-      (\<forall> \<sigma> c. weight_measure params (agreeing_validators (p, \<sigma>)) > weight_measure params (disagreeing_validators (p, \<sigma>)) \<longrightarrow> c \<in> \<epsilon> params  \<sigma> \<and> p c)"
+      (\<forall> \<sigma> \<in> \<Sigma> params. weight_measure params (agreeing_validators params (p, \<sigma>)) > weight_measure params (disagreeing_validators params (p, \<sigma>))
+        \<longrightarrow> (\<forall> c \<in> \<epsilon> params \<sigma>. p c))"
 
 (* Definition 7.14 *)
-fun later_disagreeing_validators :: "(consensus_value_property * message * validator * state) \<Rightarrow> message set"
+fun later_disagreeing_validators :: "params \<Rightarrow> (consensus_value_property * message * validator * state) \<Rightarrow> message set"
   where 
-    "later_disagreeing_validators (p, m, v, \<sigma>) = {m'. m' \<in> later_from (m, v, \<sigma>) \<and> \<not> p (est m')}"
+    "later_disagreeing_validators params (p, m, v, \<sigma>) = {m' \<in> M params. m' \<in> later_from params (m, v, \<sigma>) \<and> \<not> p (est m')}"
 
 (* Definition 7.15 *)
 (* NOTE: Define singleton set here *)
