ABOUT_CBC_PARAMS.md
@@ -1,0 +1,41 @@
+# About CBC Casper parameters
+## `params` as a global configuration
+TODO
+
+## Sets dependent on the parameters
+Isabelle don't support dependent types.
+
+Therefore, corresponding sets are defined in [CBCCasper.thy] and `message`, `state`, etc. types in function definitions are assumes that they are used for correct values.
+
+We need to take care that in these (essentially same) cases, variables need to be limited to the sets.
+
+(1) Quantify variables
+(2) Construct a set
+
+even when it's clear from the context that they belongs to a certain set.
+
+For example, here
+```
+(* Definition 4.6: Latest Message *)
+definition latest_message :: "params ⇒ state ⇒ (validator ⇒ state)"
+  where
+    "latest_message params σ v = {m ∈ M params. m ∈ from_sender params (v, σ) ∧ later_from params (m, v, σ) = ∅}"
+```
+
+However, for simplicity, we omit th
+
+About `sender`, `est` etc.
+```
+(* Definition 4.1: Observed validators *)
+definition observed :: "state ⇒ validator set"
+  where
+    "observed σ = {sender m | m. m ∈ σ}"
+```
+
+Also, `ε params σ`
+```
+(* Definition 7.12 *)
+definition is_majority_driven :: "params ⇒ consensus_value_property ⇒ bool"
+  where
+    "is_majority_driven params p = (∀ σ ∈ Σ params. is_majority params (agreeing_validators params (p, σ), σ) ⟶ (∀ c ∈ ε params σ. p c))"
+```
